proof/list_trivial_proof.v
@@ -5,12 +5,10 @@ Require Import VST.floyd.proofauto.
 Require Import VST.floyd.library.
 Require Import printer.printer_files.compiled_format.
 Require Import printer.verified_printer.Format.
+Require Import printer.verified_printer.FormatTrivial.
 Require Import Coq.Strings.Ascii.
 Require Import format_specs.
-Require Import format_std_proof.
-Require Import format_proof.
 Require Import list_specs.
-Require Import format_combinator_proof.
 
 Lemma body_clear_to_text : semax_body Vprog Gprog f_clear_to_text clear_to_text_spec.
 Proof.
@@ -61,16 +59,15 @@ Proof.
   
   Intros; destruct fs; unff listrepf.
   { Intros; unnw; vauto. }
-  Intros fst_tail_ptr fst_format_ptr.
+  Intros fst_tail_ptr fst_format_ptr format_sigma sigma_pt.
   forward.
   { entailer!; unnw; desf; entailer!. }
 
-  forward_call(fs, fst_tail_ptr, gv).
+  forward_call(fs, fst_tail_ptr, w, h, gv).
   forward.
-  { unfold mformat; Intros sigmaG pG.
-    unfold concrete_mformat; do 2 entailer. }
-  
-  unfold mformat; Intros sigmaG pG; unfold concrete_mformat.
+  { entailer; unfold concrete_mformat; entailer. }
+
+  unfold concrete_mformat.
   forward_if(
     PROP()
     LOCAL(temp _t'1 fst_format_ptr; temp _t'5 fst_tail_ptr; gvars gv; temp _fs p)
@@ -85,48 +82,223 @@ Proof.
   forward.
   { entailer; unnw; desf; entailer!. }
 
-  forward_call(sigmaG, pG, gv).
+  forward_call(format_sigma, sigma_pt, gv).
   forward.
   forward_call(t_format, fst_format_ptr, gv).
   { desf; entailer!. }
   entailer!.
 Qed.
 
-Lemma lsegf_lsegf: forall (s1 s2: list t) (x y z: val),
-  lsegf s1 x y * lsegf s2 y z |-- lsegf (s1 ++ s2) x z.
+Lemma lsegf_lsegf: forall (s1 s2: list t) (x y z: val) (w h : Z),
+  lsegf s1 x y w h * lsegf s2 y z w h |-- lsegf (s1 ++ s2) x z w h.
 Proof.
   intros s1. induction s1.
-  { intros. unff lsegf. simpl. entailer!. unnw. subst. entailer. }
-  intros. unff lsegf. Intros h y0. simpl.
+  { intros; unff lsegf; simpl; entailer!; unnw; subst; entailer. }
+  intros. 
+  unff lsegf. 
+  Intros h0 y0 format_sigma sigma_pt. 
+  simpl.
   unff lsegf.
-  Exists h y0.
+  Exists h0 y0 format_sigma sigma_pt.
   entailer!.
   apply IHs1.
 Qed.
 
-Lemma lsegf_listf (s1 s2: list t) (x y: val) :
-  lsegf s1 x y * listrepf s2 y |-- listrepf (s1 ++ s2) x.
+Lemma lsegf_listf (s1 s2: list t) (x y: val) (w h : Z):
+  lsegf s1 x y w h * listrepf s2 y w h |-- listrepf (s1 ++ s2) x w h.
 Proof.
   generalize dependent x.
   induction s1; ins; unfold lsegf.
   { entailer!; unnw; subst; entailer. }
   unff lsegf; destruct a.
-  Intros h y0.
-  unff listrepf; Exists h y0.
+  Intros h0 y0 format_sigma sigma_pt.
+  unff listrepf.
+  Exists h0 y0 format_sigma sigma_pt.
   entailer!; apply IHs1.
 Qed.
 
-Lemma lsegf_null_listrepf (sigma : list t) (p : val):
-  lsegf sigma p nullval |-- listrepf sigma p.
+Lemma lsegf_null_listrepf (sigma : list t) (p : val) (w h : Z):
+  lsegf sigma p nullval w h |-- listrepf sigma p w h.
 Proof.
   revert p.
   induction sigma.
   { unfold lsegf; unfold listrepf; entailer!. }
   unff lsegf; destruct a.
   intros p.
-  Intros h y.
+  Intros h0 y format_sigma sigma_pt.
   unff listrepf.
-  Exists h y.
+  Exists h0 y format_sigma sigma_pt.
+  entailer!.
+Qed.
+
+ Definition format_without_to_text (G : t) (x p : val) : mpred :=
+  sepcon (malloc_token Ews t_format x)
+  (data_at Ews t_format (Vint (Int.repr (Z.of_nat G.(height))),
+                        (Vint (Int.repr (Z.of_nat G.(first_line_width))),
+                         (Vint (Int.repr (Z.of_nat G.(middle_width))),
+                          (Vint (Int.repr (Z.of_nat G.(last_line_width))), p)))) x)
+.
+
+Lemma body_max_width_check : semax_body Vprog Gprog f_max_width_check max_width_check_spec.
+Proof.
+  start_function.
+  forward.
+  getnw; inv FMT_MP.
+  forward_if.
+  { forward.
+    Exists false.
+    entailer!.
+    unfold concrete_mformat.
+    entailer!. }
+  forward.
+  forward_if.
+  { forward.
+    Exists false.
+    entailer!.
+    unfold concrete_mformat.
+    entailer!. }
+  forward.
+  forward_if.
+  { forward.
+    Exists false.
+    entailer!.
+    unfold concrete_mformat.
+    entailer!. }
+  forward.
+  forward_if.
+  { forward.
+    Exists false.
+    entailer!.
+    unfold concrete_mformat.
+    entailer!. }
+  forward.
+  { entailer; unnw; desf; entailer!. }
+  forward_loop(
+    EX i : Z, EX tail : val,
+    PROP (0 <= i <= Zlength sigma;
+          Forall (fun x => fst x + Zlength (snd x) <= w) (sublist 0 i sigma))
+    LOCAL (temp _current_tail tail; temp _G p; temp _width (Vint (Int.repr w)))
+    SEP(
+      lseg (sublist 0 i sigma) sigma_pt tail;
+      listrep (sublist i (Zlength sigma) sigma) tail;
+      format_without_to_text G p sigma_pt)).
+  2: { entailer!. }
+  { Exists 0 sigma_pt.
+    entailer!.
+    { replace (sublist 0 0 sigma) with ([] : list (Z * list byte)) by list_solve.
+      list_solve. }
+    autorewrite with sublist norm.
+    unff lseg.
+    unfold format_without_to_text.
+    entailer!. }
+  2: { forward.
+    getnw; desf.
+    assert (sublist i (Zlength sigma) sigma = []) as K by auto.
+    assert (i < Zlength sigma \/ i = Zlength sigma) as KK by lia.
+    destruct KK.
+    { replace (sublist i (Zlength sigma) sigma) with
+        (Znth i sigma :: sublist (i + 1) (Zlength sigma) sigma) in K by list_solve.
+      vauto. }
+    subst.
+    autorewrite with sublist norm.
+    Exists true.
+    unff listrep.
+    unfold format_without_to_text.
+    unfold concrete_mformat.
+    entailer!.
+    { split; ins.
+      replace (sublist 0 (Zlength sigma) sigma) with sigma in * by list_solve.
+      split; vauto; lia. }
+    apply lseg_null_listrep. }
+  assert (i = Zlength sigma \/ i < Zlength sigma) as K by lia.
+  destruct K.
+  { subst.
+    autorewrite with sublist norm.
+    unff listrep.
+    Intros.
+    unnw; vauto. }
+  replace (sublist i (Zlength sigma) sigma) with
+    (Znth i sigma :: sublist (i + 1) (Zlength sigma) sigma) by list_solve.
+  unff listrep.
+  destruct (Znth i sigma) as (ith_shift, ith_line) eqn:E.
+  Intros ith_tail_ptr ith_line_ptr.
+  forward.
+  forward_call(Ews, ith_line, ith_line_ptr).
+  forward.
+  forward_if.
+  { forward.
+    Exists false.
+    entailer!.
+    { split; ins; desf.
+      assert ((fun x : Z * list byte => fst x + Zlength (snd x) <= w) (Znth i sigma)) as K1.
+      { apply Forall_Znth; auto; lia. }
+      assert ((fun x : Z * list byte => 0 <= fst x + Zlength (snd x) <= Int.max_unsigned) (Znth i sigma)) as K2.
+      { apply Forall_Znth; auto; lia. }
+      rewrite E in *; ins.
+      autorewrite with sublist norm in *.
+      lia. }
+    unfold concrete_mformat.
+    unfold format_without_to_text.
+    entailer!.
+    assert (
+      lseg (sublist 0 (i + 1) sigma) sigma_pt ith_tail_ptr *
+      listrep (sublist (i + 1) (Zlength sigma) sigma) ith_tail_ptr |--
+      listrep sigma sigma_pt
+    ) as K.
+    { assert(sigma = (sublist 0 (i + 1) sigma ++ sublist (i + 1) (Zlength sigma) sigma)) as K by list_solve.
+      rewrite K at 4.
+      apply lseg_list. }
+    eapply derives_trans.
+    2: eauto.
+    entailer!.
+    assert(
+      lseg (sublist 0 i sigma) sigma_pt tail *
+      lseg [Znth i sigma] tail ith_tail_ptr |--
+      lseg (sublist 0 (i + 1) sigma) sigma_pt ith_tail_ptr
+    ) as F.
+    { replace (sublist 0 (i + 1) sigma) with
+        (sublist 0 i sigma ++ [Znth i sigma]) by list_solve.
+      apply lseg_lseg. }
+    eapply derives_trans.
+    2: eauto.
+    entailer!.
+    unff lseg.
+    rewrite E.
+    Exists ith_tail_ptr ith_line_ptr.
+    entailer!. }
+  forward.
+  { entailer!.
+    unnw; desf. } 
+  Exists ((i + 1), ith_tail_ptr).
+  assert ((fun x : Z * list byte => 0 <= fst x + Zlength (snd x) <= Int.max_unsigned) (Znth i sigma)) as K2.
+  { apply Forall_Znth; auto; lia. }
+  entailer!.
+  { split.
+    { lia. }
+    replace (sublist 0 (i + 1) sigma) with
+      (sublist 0 i sigma ++ [Znth i sigma]) by list_solve.
+    apply Forall_app; split; vauto.
+    rewrite E in *.
+    ins.
+    autorewrite with sublist norm in *.
+    apply Forall_cons.
+    2: apply Forall_nil.
+    ins; lia. }
+  entailer!.
+  assert(
+    lseg (sublist 0 i sigma) sigma_pt tail *
+    lseg [Znth i sigma] tail ith_tail_ptr |--
+    lseg (sublist 0 (i + 1) sigma) sigma_pt ith_tail_ptr
+  ) as F.
+  { replace (sublist 0 (i + 1) sigma) with
+      (sublist 0 i sigma ++ [Znth i sigma]) by list_solve.
+    apply lseg_lseg. }
+  eapply derives_trans.
+  2: eauto.
+  entailer!.
+  unff lseg.
+  rewrite E.
+  Exists ith_tail_ptr ith_line_ptr.
   entailer!.
 Qed.
 
@@ -176,6 +348,74 @@ Proof.
   vauto.
 Qed.
 
+Lemma beside_doc_app_l (l1 l2: list t) (w : Z) (G : t):
+  FormatTrivial.besideDoc (Z.to_nat w) l1 [G] ++
+    FormatTrivial.besideDoc (Z.to_nat w) l2 [G] =
+      FormatTrivial.besideDoc (Z.to_nat w) (l1 ++ l2) [G].
+Proof.
+  unfold FormatTrivial.besideDoc.
+  unfold FormatTrivial.cross_general.
+  repeat rewrite <- filter_app.
+  repeat rewrite <- concat_app.
+  repeat rewrite map_cons.
+  repeat rewrite map_nil.
+  repeat rewrite concat_app.
+  repeat rewrite concat_cons.
+  repeat rewrite concat_nil.
+  autorewrite with sublist norm.
+  repeat rewrite filter_app.
+  repeat rewrite map_app.
+  repeat rewrite filter_app.
+  vauto.
+Qed.
+
+Lemma beside_doc_llw_add (fs : list (Z * list byte)) (llw w : Z):
+  0 <= 8 * w <= Int.max_unsigned - 1 ->
+  Forall (fun x => 0 <= 4 * (fst x) <= Int.max_unsigned - 1) fs ->
+  Forall (fun x => 0 <= 4 * (Zlength (snd x)) + 1 <= Int.max_unsigned) fs ->
+  Forall (fun x => 0 <= fst x + Zlength (snd x) <= w) fs ->
+  0 <= llw <= w ->
+  Forall (fun x => 0 <= 4 * (fst x + llw) <= Int.max_unsigned - 1) fs.
+Proof.
+  ins.
+  induction fs.
+  { apply Forall_nil. }
+  apply Forall_cons_iff in H0.
+  destruct H0.
+  apply Forall_cons_iff in H1.
+  destruct H1.
+  apply Forall_cons_iff in H2.
+  destruct H2.
+  apply Forall_cons.
+  2: apply (IHfs H4 H5 H6 ).
+  lia.
+Qed.
+
+Lemma beside_doc_ab_pred (G F : t) (fs1 fs2 : list (Z * list byte)) (w : Z):
+  0 <= 8 * w <= Int.max_unsigned - 1 ->
+  list_mp fs1 ->
+  Forall (fun x => 0 <= fst x + Zlength (snd x) <= w) fs2 ->
+  Forall (fun x => 0 <= fst x + Zlength (snd x) <= w) fs1 ->
+  to_text_add_beside_pred G F fs1 fs2.
+Proof.
+  ins.
+  unfold to_text_add_beside_pred.
+  desf.
+  induction fs1.
+  { apply Forall_nil. }
+  inv H1.
+  inv H0.
+  inv H2.
+  apply Forall_cons_iff in  list_mp_forall_fst.
+  apply Forall_cons_iff in  list_mp_forall_snd.
+  desf.
+  apply Forall_cons.
+  2: { apply IHfs1; vauto. 
+       apply mk_list_mp; vauto.
+       list_solve. }
+  unfold Int.max_unsigned; ins.
+  lia.
+Qed.
 
 Lemma body_beside_doc : semax_body Vprog Gprog f_beside_doc beside_doc_spec.
 Proof.
@@ -184,8 +424,8 @@ Proof.
   { forward_if(
     PROP ( )
     LOCAL (gvars gv; temp _width (Vint (Int.repr w)); temp _height (Vint (Int.repr h)); temp _fs1 p1; temp _fs2 p2)
-    SEP (listrepf fs1 p1; mem_mgr gv)).
-    { forward_call(fs2, p2, gv); entailer!. }
+    SEP (listrepf fs1 p1 w h; mem_mgr gv)).
+    { forward_call(fs2, p2, w, h, gv); entailer!. }
     { forward; entailer!. 
       unnw; desf.
       assert (fs2 = []) by auto; subst.
@@ -200,7 +440,7 @@ Proof.
   { forward; entailer!. }
 
   forward_if(p2 <> nullval).
-  { forward_call(fs1, p1, gv).
+  { forward_call(fs1, p1, w, h, gv).
     forward.
     unnw; desf.
     assert (fs2 = []) by auto; subst.
@@ -224,9 +464,9 @@ Proof.
             temp _has_item (Val.of_bool (0 <? Zlength res_part)); temp _result result_ptr; gvars gv; 
             temp _width (Vint (Int.repr w)); temp _height (Vint (Int.repr h));
             temp _fs1 p1; temp _fs2 p2; temp _result_tail result_tail_ptr)
-      SEP (mem_mgr gv; listrepf fs1 p1; lsegf (sublist 0 i fs2) p2 head_ptr; 
-          listrepf (sublist i (Zlength fs2) fs2) head_ptr; lsegf res_part result_ptr result_tail_ptr;
-          listrepf [empty] result_tail_ptr)) as loop_invariant eqn:eqn_loop.
+      SEP (mem_mgr gv; listrepf fs1 p1 w h; lsegf (sublist 0 i fs2) p2 head_ptr w h; 
+          listrepf (sublist i (Zlength fs2) fs2) head_ptr w h; lsegf res_part result_ptr result_tail_ptr w h;
+          listrepf [empty] result_tail_ptr w h)) as loop_invariant eqn:eqn_loop.
   remember (
       EX result_tail_ptr : val, EX res_part : list t,
       PROP(res_part = filter (fun G => (G.(height) <=? Z.to_nat h)%nat) (FormatTrivial.besideDoc (Z.to_nat w) fs1 fs2))
@@ -234,8 +474,8 @@ Proof.
             temp _result_tail result_tail_ptr;
             temp _width (Vint (Int.repr w)); temp _height (Vint (Int.repr h));
             temp _fs1 p1; temp _fs2 p2)
-      SEP (mem_mgr gv; listrepf fs1 p1; listrepf fs2 p2; lsegf res_part result_ptr result_tail_ptr;
-          listrepf [empty] result_tail_ptr)) as break_invariant eqn:eqn_break.
+      SEP (mem_mgr gv; listrepf fs1 p1 w h; listrepf fs2 p2 w h; lsegf res_part result_ptr result_tail_ptr w h;
+          listrepf [empty] result_tail_ptr w h)) as break_invariant eqn:eqn_break.
   forward_loop(loop_invariant) break: (break_invariant).
   { subst.
     Exists 0 p2 result_ptr ([] : list t).
@@ -245,29 +485,36 @@ Proof.
     { rewrite sublist_skip; vauto. }
     rewrite K.
     unff lsegf; entailer!; ins.
+    unfold mformat.
+    Intros sigma_list sigma_pt.
     unff listrepf.
-    Exists nullval cur_empty_ptr.
-    entailer!. }
+    Exists nullval cur_empty_ptr sigma_list sigma_pt.
+    unfold concrete_mformat.
+    entailer!.
+    getnw.
+    inv FMT_MP.
+    unfold empty in *; ins.
+    unnw; unfold good_format; ins.
+    assert (sigma_list = []) by list_solve; subst.
+    list_solve. }
   2: { subst.
       Intros result_tail_ptr res_part.
-      forward_call(fs1, p1, gv).
-      forward_call(fs2, p2, gv).
+      forward_call(fs1, p1, w, h, gv).
+      forward_call(fs2, p2, w, h, gv).
       forward_if (
         Zlength res_part <> 0
       ).
       { destruct (0 <? Zlength res_part) eqn:E; vauto.
-        forward_call([empty], result_ptr, gv).
+        forward_call([empty], result_ptr, w, h, gv).
         { desf; entailer!.
           replace ((filter (fun G : t => (height G <=? Z.to_nat h)%nat)
           (FormatTrivial.besideDoc (Z.to_nat w) fs1 fs2))) with ([] : list t) by list_solve.
           unff lsegf; unff listrepf.
           entailer!; subst; unnw; entailer!.
-          Exists nullval y; entailer!. }
+          Exists nullval y format_sigma sigma_pt; entailer!. }
         forward.
         Exists nullval ([] : list t); entailer!.
         2: { unff listrepf; entailer!. }
-        split.
-        { unfold good_format_list; vauto. }
         list_solve. }
       { forward; entailer!; ins.
         assert (Zlength (filter (fun G : t => (height G <=? Z.to_nat h)%nat)
@@ -279,15 +526,15 @@ Proof.
         PROP(0 <= i < Zlength res_part)
         LOCAL(temp _new_result_tail new_result_tail; temp _fs1 p1; temp _fs2 p2; 
               temp _result_tail result_tail_ptr; gvars gv; temp _result result_ptr)
-        SEP(mem_mgr gv; lsegf (sublist 0 i res_part) result_ptr new_result_tail; 
-            listrepf (sublist i (Zlength res_part) res_part ++ [empty]) new_result_tail)
+        SEP(mem_mgr gv; lsegf (sublist 0 i res_part) result_ptr new_result_tail w h; 
+            listrepf (sublist i (Zlength res_part) res_part ++ [empty]) new_result_tail w h)
       ) break: (
         EX new_result_tail : val,
         PROP()
         LOCAL(temp _new_result_tail new_result_tail; temp _fs1 p1; temp _fs2 p2; 
               temp _result_tail result_tail_ptr; gvars gv; temp _result result_ptr)
-        SEP(mem_mgr gv; lsegf (sublist 0 (Zlength res_part - 1) res_part) result_ptr new_result_tail; 
-            listrepf (sublist (Zlength res_part - 1) (Zlength res_part) res_part ++ [empty]) new_result_tail)).
+        SEP(mem_mgr gv; lsegf (sublist 0 (Zlength res_part - 1) res_part) result_ptr new_result_tail w h; 
+            listrepf (sublist (Zlength res_part - 1) (Zlength res_part) res_part ++ [empty]) new_result_tail w h)).
       { Exists 0 result_ptr.
         entailer!.
         autorewrite with sublist.
@@ -301,7 +548,7 @@ Proof.
             :: sublist (i + 1) (Zlength res_part) res_part) ++ [empty]) with
             (Znth i res_part :: (sublist (i + 1) (Zlength res_part) res_part ++ [empty])) by list_solve.
         unff listrepf.
-        Intros ith_tail_ptr ith_format_ptr.
+        Intros ith_tail_ptr ith_format_ptr format_sigma sigma_pt.
         forward.
         { entailer!; getnw; desf. }
         assert (i + 1 = Zlength res_part \/ i + 1 < Zlength res_part) as K by lia.
@@ -309,31 +556,32 @@ Proof.
         { replace (sublist (i + 1) (Zlength res_part) res_part) with ([] : list t) by list_solve.
           autorewrite with sublist.
           unff listrepf.
-          Intros nullval_tail_ptr empty_ptr.
+          Intros nullval_tail_ptr empty_ptr format_sigma_empty sigma_pt_empty.
           forward.
           { unnw; subst; entailer!. }
           getnw; rewrite LIST_NULL_PTR.
           forward_if.
           { vauto. }
           forward.  
-          Exists new_result_tail_ptr.
           entailer!.
+          Exists new_result_tail_ptr.
           remember (filter (fun G : t => (height G <=? Z.to_nat h)%nat) (FormatTrivial.besideDoc (Z.to_nat w) fs1 fs2))
             as res_part.
           replace i with (Zlength res_part - 1) by lia.
           replace (sublist (Zlength res_part - 1) (Zlength res_part) res_part ++ [empty])
             with [Znth (Zlength res_part - 1) res_part; empty] by list_solve.
           unff listrepf.
-          Exists ith_tail_ptr ith_format_ptr.
-          Exists nullval empty_ptr.
+          Exists ith_tail_ptr ith_format_ptr format_sigma sigma_pt.
+          Exists nullval empty_ptr format_sigma_empty sigma_pt_empty.
           entailer!.
-        }
+          unnw.
+          list_solve. }
         replace (sublist (i + 1) (Zlength res_part) res_part)
           with (Znth (i + 1) res_part :: sublist (i + 2) (Zlength res_part) res_part) by list_solve.
         replace ((Znth (i + 1) res_part :: sublist (i + 2) (Zlength res_part) res_part) ++ [empty]) with
             (Znth (i + 1) res_part :: ((sublist (i + 2) (Zlength res_part) res_part ++ [empty]))) by list_solve.
         unff listrepf.
-        Intros ithplus_tail_ptr ithplus_format_ptr.
+        Intros ithplus_tail_ptr ithplus_format_ptr ith_plus_sigma ith_plus_sigma_pt.
         forward.
         { entailer!; unnw; desf.  }
         forward_if.
@@ -345,67 +593,60 @@ Proof.
           replace ((Znth (i + 1) l :: sublist (i + 2) (Zlength l) l) ++ [empty]) with 
               (Znth (i + 1) l :: (sublist (i + 2) (Zlength l) l ++ [empty])) by list_solve.
           unff listrepf.
-          Exists ithplus_tail_ptr ithplus_format_ptr.
+          Exists ithplus_tail_ptr ithplus_format_ptr ith_plus_sigma ith_plus_sigma_pt.
           entailer!.
           remember (filter (fun G : t => (height G <=? Z.to_nat h)%nat) (FormatTrivial.besideDoc (Z.to_nat w) fs1 fs2)).
           assert (
-            lsegf (sublist 0 i l) result_ptr new_result_tail_ptr *
-            lsegf [Znth i l] new_result_tail_ptr ith_tail_ptr |--
-            lsegf (sublist 0 (i + 1) l) result_ptr ith_tail_ptr) as K.
+            lsegf (sublist 0 i l) result_ptr new_result_tail_ptr w h *
+            lsegf [Znth i l] new_result_tail_ptr ith_tail_ptr w h |--
+            lsegf (sublist 0 (i + 1) l) result_ptr ith_tail_ptr w h) as K.
           { replace (sublist 0 (i + 1) l) with (sublist 0 i l ++ [Znth i l]) by list_solve.
             eapply lsegf_lsegf. }
           eapply derives_trans.
           2: eauto.
           entailer!.
-          unff lsegf; Exists ith_tail_ptr ith_format_ptr.
+          unff lsegf; Exists ith_tail_ptr ith_format_ptr format_sigma sigma_pt.
           entailer!. }
         forward.
         replace ithplus_tail_ptr with nullval by vauto.
         destruct (sublist (i + 2) (Zlength res_part) res_part).
         { autorewrite with sublist norm.
           unff listrepf.
-          Intros x y.
+          Intros x y format_sigma0 sigma_pt0.
           entailer!. }
         replace (((t :: l) ++ [empty])) with (t :: (l ++ [empty])) by list_solve.
         unff listrepf.
-        Intros x y.
+        Intros x y format_sigma0 sigma_pt0.
         entailer!. }
     Intros new_result_tail.
     replace (sublist (Zlength res_part - 1) (Zlength res_part) res_part ++ [empty]) with 
         [Znth (Zlength res_part - 1) res_part; empty] by list_solve.
     unff listrepf.
-    Intros empty_list_ptr last_format_ptr nullval_ptr empty_format_ptr.
+    Intros empty_list_ptr last_format_ptr empty_sigma empty_sigma_ptr.
+    Intros nullval_ptr empty_format_ptr format_sigma0 sigma_pt0.
     forward.
-    forward_call([empty], empty_list_ptr, gv).
+    forward_call([empty], empty_list_ptr, w, h, gv).
     { getnw; subst.
       unff listrepf.
-      Exists nullval empty_format_ptr.
+      Exists nullval empty_format_ptr format_sigma0 sigma_pt0.
       entailer!. }
     do 2 forward.
     Exists result_ptr (filter (fun G : t => (height G <=? Z.to_nat h)%nat) (FormatTrivial.besideDoc (Z.to_nat w) fs1 fs2)).
     entailer!.
-    2: {
-      remember (filter (fun G : t => (height G <=? Z.to_nat h)%nat) (FormatTrivial.besideDoc (Z.to_nat w) fs1 fs2)).
-      assert (
-        lsegf (sublist 0 (Zlength l - 1) l) result_ptr new_result_tail *
-        listrepf [Znth (Zlength l - 1) l] new_result_tail |--
-        listrepf l result_ptr
-      ) as K.
-      { assert(l = (sublist 0 (Zlength l - 1) l ++ [Znth (Zlength l - 1) l])) as KK by list_solve.
-        rewrite KK at 5.
-        apply lsegf_listf. }
-      eapply derives_trans.
-      2: eauto.
-      unff listrepf.
-      Exists nullval last_format_ptr.
-      entailer!. }
-    unfold good_format_list.
-    unfold good_format.
-    eapply Forall_and.
-    2: { apply beside_doc_forall_height. }
-    unfold FormatTrivial.besideDoc.
-    unfold FormatTrivial.cross_general.
-    apply beside_doc_forall_width. }
+    remember (filter (fun G : t => (height G <=? Z.to_nat h)%nat) (FormatTrivial.besideDoc (Z.to_nat w) fs1 fs2)).
+    assert (
+      lsegf (sublist 0 (Zlength l - 1) l) result_ptr new_result_tail w h *
+      listrepf [Znth (Zlength l - 1) l] new_result_tail w h |--
+      listrepf l result_ptr w h
+    ) as K.
+    { assert(l = (sublist 0 (Zlength l - 1) l ++ [Znth (Zlength l - 1) l])) as KK by list_solve.
+      rewrite KK at 5.
+      apply lsegf_listf. }
+    eapply derives_trans.
+    2: eauto.
+    unff listrepf.
+    Exists nullval last_format_ptr empty_sigma empty_sigma_ptr.
+    entailer!. }
 subst.
 Intros i head_ptr result_tail_ptr res_part.
 forward_if.
@@ -437,12 +678,12 @@ remember (
           temp _width (Vint (Int.repr w)); temp _height (Vint (Int.repr h));
           temp _fs1 p1; temp _fs2 p2; temp _result_tail result_tail_ptr_new)
     SEP (mem_mgr gv; 
-        lsegf (sublist 0 j fs1) p1 head_ptr2;
-        listrepf (sublist j (Zlength fs1) fs1) head_ptr2;
-        lsegf (sublist 0 i fs2) p2 head_ptr; 
-        listrepf (sublist i (Zlength fs2) fs2) head_ptr; 
-        lsegf res_part_new result_ptr result_tail_ptr_new;
-        listrepf [empty] result_tail_ptr_new)) as loop_invariant eqn:eqn_loop.
+        lsegf (sublist 0 j fs1) p1 head_ptr2 w h;
+        listrepf (sublist j (Zlength fs1) fs1) head_ptr2 w h;
+        lsegf (sublist 0 i fs2) p2 head_ptr w h; 
+        listrepf (sublist i (Zlength fs2) fs2) head_ptr w h; 
+        lsegf res_part_new result_ptr result_tail_ptr_new w h;
+        listrepf [empty] result_tail_ptr_new w h)) as loop_invariant eqn:eqn_loop.
 remember (
     EX result_tail_ptr_new : val, EX res_part_new : list t,
     PROP(res_part_new = filter (fun G => (G.(height) <=? Z.to_nat h)%nat) (FormatTrivial.besideDoc (Z.to_nat w) fs1 (sublist 0 (i + 1) fs2)))
@@ -454,11 +695,11 @@ remember (
           temp _fs1 p1; temp _fs2 p2;
           temp _fs2_tail head_ptr)
     SEP (mem_mgr gv; 
-        listrepf fs1 p1; 
-        lsegf (sublist 0 i fs2) p2 head_ptr; 
-        listrepf (sublist i (Zlength fs2) fs2) head_ptr; 
-        lsegf res_part_new result_ptr result_tail_ptr_new;
-        listrepf [empty] result_tail_ptr_new)) as break_invariant eqn:eqn_break.
+        listrepf fs1 p1 w h; 
+        lsegf (sublist 0 i fs2) p2 head_ptr w h; 
+        listrepf (sublist i (Zlength fs2) fs2) head_ptr w h; 
+        lsegf res_part_new result_ptr result_tail_ptr_new w h;
+        listrepf [empty] result_tail_ptr_new w h)) as break_invariant eqn:eqn_break.
 forward_loop(loop_invariant) break: (break_invariant).
 { rewrite eqn_loop.
   Exists 0 p1 result_tail_ptr res_part.
@@ -478,20 +719,20 @@ forward_loop(loop_invariant) break: (break_invariant).
   replace (sublist i (Zlength fs2) fs2) 
     with (Znth i fs2 :: (sublist (i + 1) (Zlength fs2) fs2)) by list_solve.
   unff listrepf.
-  Intros ith_tail_ptr ith_format_ptr.
-  Intros nullval_ptr empty_ptr.
+  Intros ith_tail_ptr ith_format_ptr ith_sigma ith_sigma_pt.
+  Intros nullval_ptr empty_ptr empty_sigma empty_sigma_pt.
   getnw; rewrite LIST_NULL_PTR.
   forward.
   { entailer!; unnw; desf. }
   Exists (i + 1) ith_tail_ptr result_tail_ptr_new res_part_new.
   entailer!.
   unff listrepf.
-  Exists nullval empty_ptr.
+  Exists nullval empty_ptr empty_sigma empty_sigma_pt.
   entailer!.
   assert (
-    lsegf (sublist 0 i fs2) p2 head_ptr *
-    lsegf [Znth i fs2] head_ptr ith_tail_ptr |--
-    lsegf (sublist 0 (i + 1) fs2) p2 ith_tail_ptr
+    lsegf (sublist 0 i fs2) p2 head_ptr w h *
+    lsegf [Znth i fs2] head_ptr ith_tail_ptr w h |--
+    lsegf (sublist 0 (i + 1) fs2) p2 ith_tail_ptr w h
   ) as K.
   { replace (sublist 0 (i + 1) fs2) with
       (sublist 0 i fs2 ++ [Znth i fs2]) by list_solve.
@@ -500,7 +741,7 @@ forward_loop(loop_invariant) break: (break_invariant).
   2: eauto.
   entailer!.
   unff lsegf; entailer!.
-  Exists ith_tail_ptr ith_format_ptr.
+  Exists ith_tail_ptr ith_format_ptr ith_sigma ith_sigma_pt.
   entailer!. }
 rewrite eqn_loop.
 Intros j head_ptr2 result_tail_ptr_new res_part_new.
@@ -560,51 +801,113 @@ replace (sublist i (Zlength fs2) fs2) with
 replace (sublist j (Zlength fs1) fs1) with
   (Znth j fs1 :: (sublist (j + 1) (Zlength fs1) fs1)) by list_solve.
 unff listrepf.
-Intros ith_tail_fs1_ptr ith_format_fs1_ptr.
-Intros ith_tail_fs2_ptr ith_format_fs2_ptr.
-Intros nullval_ptr empty_ptr.
+Intros ith_tail_fs1_ptr ith_format_fs1_ptr fs1_sigma fs1_sigma_pt.
+Intros ith_tail_fs2_ptr ith_format_fs2_ptr fs2_sigma fs2_sigma_pt.
+Intros nullval_ptr empty_ptr empty_sigma empty_sigma_pt.
 getnw; rewrite LIST_NULL_PTR.
 forward.
 { entailer.
-  unfold mformat.
   unfold concrete_mformat.
-  Intros x y x1 y1 x2 y2.
   entailer!. }
 forward.
 { entailer.
-  unfold mformat.
   unfold concrete_mformat.
-  Intros x y x1 y1 x2 y2.
   entailer!. }
-unfold mformat.
-Intros sigmaG pG sigmaF pF sigmaEmpty pEmpty.
 unfold concrete_mformat.
 Intros.
 forward_call(Znth j fs1, Znth i fs2, 
-    ith_format_fs1_ptr, ith_format_fs2_ptr, sigmaG, sigmaF, pG, pF, gv).
+    ith_format_fs1_ptr, ith_format_fs2_ptr, fs1_sigma, fs2_sigma, fs1_sigma_pt, fs2_sigma_pt, gv).
 { unfold concrete_mformat; entailer!. }
-{ split.
-  { getnw; inv FMT_MP.
-    getnw; inv FMT_MP.
-    getnw; inv FMT_MP.
-    unfold good_format_list in *.
-    assert (good_format (Znth j fs1) w h) as GF1.
-    { list_solve. }
-    assert (good_format (Znth i fs2) w h) as GF2.
-    { list_solve. }
-    unfold good_format in GF1.
-    unfold good_format in GF2.
-    desc.
-    unfold total_width in *; ins.
-    destruct (Znth j fs1).
-    destruct (Znth i fs2).
-    apply mk_format_comb; ins; try lia.
-    unfold Int.max_unsigned in *; ins; lia. }
+{ getnw; inv FMT_MP; inv GOOD_FORMAT.
+  getnw; inv FMT_MP; inv GOOD_FORMAT.
+  getnw; inv FMT_MP; inv GOOD_FORMAT.  
+  desf.
   split.
-  { getnw
-
-  }
+  { apply mk_format_comb; try lia. }
+  split.
+  { eapply beside_doc_llw_add.
+    4: eauto.
+    { lia. }
+    3: lia.
+    all: inv format_mp_list_mp0.
+    all: vauto. }
+  eapply beside_doc_ab_pred.
+  4: eauto.
+  { lia. }
+  all: vauto. }
+Intros vret.
+destruct vret as (vret_sigma, result_sigma_pt).
+destruct vret_sigma as (result_format_ptr, result_sigma).
+forward.
+unfold concrete_mformat.
+Intros.
+forward_call(add_beside (Znth j fs1) (Znth i fs2), result_format_ptr, result_sigma, result_sigma_pt, w, h).
+{ unfold concrete_mformat.
+  entailer!.
+  entailer!. }
+Intros width_check_result.
+forward_if(
+  EX res_part_new : list t, EX result_tail_ptr_new : val,
+  PROP(0 <= j <= Zlength fs1;
+        res_part_new = res_part ++ filter (fun G => (G.(height) <=? Z.to_nat h)%nat) (FormatTrivial.besideDoc (Z.to_nat w) (sublist 0 (j + 1) fs1) [Znth i fs2]))
+  LOCAL(temp _fs2_tail head_ptr; temp _fs1_tail head_ptr2;
+        temp _has_item (Val.of_bool (0 <? Zlength res_part_new)); 
+        temp _result result_ptr; gvars gv; 
+        temp _width (Vint (Int.repr w)); temp _height (Vint (Int.repr h));
+        temp _fs1 p1; temp _fs2 p2; temp _result_tail result_tail_ptr_new)
+  SEP (mem_mgr gv; 
+      lsegf (sublist 0 j fs1) p1 head_ptr2 w h;
+      listrepf (sublist j (Zlength fs1) fs1) head_ptr2 w h;
+      lsegf (sublist 0 i fs2) p2 head_ptr w h; 
+      listrepf (sublist i (Zlength fs2) fs2) head_ptr w h; 
+      lsegf res_part_new result_ptr result_tail_ptr_new w h;
+      listrepf [empty] result_tail_ptr_new w h;
+      concrete_mformat (add_beside (Znth j fs1) (Znth i fs2)) result_format_ptr result_sigma result_sigma_pt)).
+2: { forward; entailer!.
+     Exists ((filter (fun G : t => (height G <=? Z.to_nat h)%nat)
+              (besideDoc (Z.to_nat w) fs1 (sublist 0 i fs2)) ++
+              filter (fun G : t => (height G <=? Z.to_nat h)%nat)
+              (besideDoc (Z.to_nat w) (sublist 0 j fs1) [Znth i fs2]))) result_tail_ptr_new; entailer!.
+     2: {
+        unff listrepf.
+        Exists nullval empty_ptr empty_sigma empty_sigma_pt.
+        entailer!.  
+        unff concrete_mformat.
+        entailer!.
+        replace (sublist j (Zlength fs1) fs1) with 
+          (Znth j fs1 :: sublist (j + 1) (Zlength fs1) fs1) by list_solve.
+        unff listrepf.
+        Exists ith_tail_fs1_ptr ith_format_fs1_ptr fs1_sigma fs1_sigma_pt.
+        unfold concrete_mformat.
+        entailer!.
+        replace (sublist i (Zlength fs2) fs2) with 
+          (Znth i fs2 :: sublist (i + 1) (Zlength fs2) fs2) by list_solve.
+        unff listrepf.
+        Exists ith_tail_fs2_ptr ith_format_fs2_ptr fs2_sigma fs2_sigma_pt.
+        unfold concrete_mformat.
+        entailer!. }
+    replace (sublist 0 (j + 1) fs1) with (sublist 0 j fs1 ++ [Znth j fs1]) by list_solve.
+    rewrite <- beside_doc_app_l.
+    apply app_inv_head_iff.
+    rewrite filter_app.
+    enough(
+      filter (fun G : t => (height G <=? Z.to_nat h)%nat) (besideDoc (Z.to_nat w) [Znth j fs1] [Znth i fs2]) = []
+    ) as K.
+    { rewrite K; list_solve. }
+    unfold FormatTrivial.besideDoc.
+    unfold FormatTrivial.cross_general.
+    rewrite map_cons.
+    rewrite concat_cons.
+    rewrite map_nil.
+    rewrite concat_nil.
+    autorewrite with sublist norm.
+    
 }
-
+2: {
+  forward.
+  { entailer!; unnw; desf. }
+  rewrite eqn_loop.
+  Exists (j + 1) ith_tail_fs1_ptr result_tail_ptr_new 
+}
 
 Admitted.
