proof/format_proof.v
@@ -6,7 +6,6 @@ Require Import printer.printer_files.compiled_format.
 Require Import printer.verified_printer.Format.
 Require Import Coq.Strings.Ascii.
 Require Import format_specs.
-Require Import format_std_proof.
 Require Import list_specs.
 
 Lemma less_components_fact1: 
